schedule.md
@@ -6,16 +6,16 @@ permalink: /schedule/
 
 | # | Topic | Dates | Materials | Comments | 
 |--:|-------|-------|-----------|----------|
-| 1 | First day of class | 13/01 | [slides(key)]({{site.baseurl}}/lectures/0_first_day_of_classes.key), [slides (pdf)]({{site.baseurl}}/lectures/0_first_day_of_classes.pdf) | [Lambda, the Ultimate TA](https://vimeo.com/6615365) |
+| 1 | First day of class | 13/01 | [slides (key)]({{site.baseurl}}/lectures/0_first_day_of_classes.key), [slides (pdf)]({{site.baseurl}}/lectures/0_first_day_of_classes.pdf) | [Lambda, the Ultimate TA](https://vimeo.com/6615365) |
 | 2 | Functional Programming in Coq | 14/01, 16/01 | [Coq]({{site.baseurl}}/lectures/FunctionalProgramming.v), [notes]({{site.baseurl}}/lectures/FunctionalProgramming.html) | |
 | 3 | Logic | 16/01, 20/01, 21/01, 22/01 | [Coq]({{site.baseurl}}/lectures/Logic.v), [notes]({{site.baseurl}}/lectures/Logic.html) | [Proposition as Types](https://www.youtube.com/watch?v=IOiZatlZtGU) |
 | 4 | Induction | 23/01, 27/01, 28/01 | [Coq]({{site.baseurl}}/lectures/Induction.v), [notes]({{site.baseurl}}/lectures/Induction.html) | |
 | 5 | BasicSyntax | 29/01, 30/01 | [Coq]({{site.baseurl}}/lectures/BasicSyntax.v) | |
 | 6 | Interpreters | 03/02, 04,02, 05/02 | [Coq]({{site.baseurl}}/lectures/Interpreters.v) | |
 | 7 | Logic Programming | 05/02, 06/02  | [Coq]({{site.baseurl}}/lectures/LogicProgramming.v) | |
-| 8 | Transition Systems | 10/2 + tutorial, 11/2, 12/2, 13/2, 17/2 + tutorial, 18/2 | [Coq]({{site.baseurl}}/lectures/TransitionSystems.v), [slides(key)]({{site.baseurl}}/lectures/2_transition_systems.key), [slides (pdf)]({{site.baseurl}}/lectures/2_transition_systems.pdf) | |
-| 9 | Operational Semantics | 19/2, 20/2, 24/2 (only tutorial), 25/2 (only tutorial), 26/2, 27/2, 02/03 (only tutorial), 03/03, 05/03, tutorial (36 min of video released on 1/4; Pset7 opsem solutions) | [Coq]({{site.baseurl}}/lectures/OperationalSemantics.v), [slides(key)]({{site.baseurl}}/lectures/3_operational_semantics.key), [slides (pdf)]({{site.baseurl}}/lectures/3_operational_semantics.pdf) | |
-| 10 | Lambda Calculus | 05/03, 09/03 + tutorial, 11/03, 12/03, 16/03, 66 min of videos released on 31/3, tutorial (38 min of video released on 1/4; subtyping) | [Coq]({{site.baseurl}}/lectures/LambdaCalculus.v), [slides(key)]({{site.baseurl}}/lectures/4_lambda_calculus.key), [slides (pdf)]({{site.baseurl}}/lectures/2_lambda_calculus.pdf) | |
+| 8 | Transition Systems | 10/2 + tutorial, 11/2, 12/2, 13/2, 17/2 + tutorial, 18/2 | [Coq]({{site.baseurl}}/lectures/TransitionSystems.v), [slides (key)]({{site.baseurl}}/lectures/2_transition_systems.key), [slides (pdf)]({{site.baseurl}}/lectures/2_transition_systems.pdf) | |
+| 9 | Operational Semantics | 19/2, 20/2, 24/2 (only tutorial), 25/2 (only tutorial), 26/2, 27/2, 02/03 (only tutorial), 03/03, 05/03, tutorial (36 min of video released on 1/4; Pset7 opsem solutions) | [Coq]({{site.baseurl}}/lectures/OperationalSemantics.v), [slides (key)]({{site.baseurl}}/lectures/3_operational_semantics.key), [slides (pdf)]({{site.baseurl}}/lectures/3_operational_semantics.pdf) | |
+| 10 | Lambda Calculus | 05/03, 09/03 + tutorial, 11/03, 12/03, 16/03, 66 min of videos released on 31/3, tutorial (38 min of video released on 1/4; subtyping) | [Coq]({{site.baseurl}}/lectures/LambdaCalculus.v), [slides (key)]({{site.baseurl}}/lectures/4_lambda_calculus.key), [slides (pdf)]({{site.baseurl}}/lectures/2_lambda_calculus.pdf) | |
 | 11 | Hoare Logic | | [Coq]({{site.baseurl}}/lectures/HoareLogic.v) | |
 | 12 | Functional Programming in F\* | | [slides(pdf)]({{site.baseurl}}/lectures/1_fstar_functional_programming.key), [fst]({{site.baseurl}}/lectures/fstar_functional.fst) | |
 | 13 | Verifying Functional Programs in F\* | | [fst]({{site.baseurl}}/lectures/fstar_verification.fst) | |
